SPos/Typing/Substitution.lean
@@ -9,7 +9,7 @@ theorem Subst.WellTyped.lift {σ : Subst n m} (hσ : Subst.WellTyped σ Γ Δ) {
   rcases hlook.inv rfl with ⟨rfl, rfl⟩ | ⟨j, τ', rfl, rfl, hj⟩
   · have h0 : Subst.lift σ 0 = Tm.var 0 := by simp [Subst.lift]
     rw [h0, Tm.weaken_subst]
-    exact .var hΔτ Lookup.here
+    exact DefEq.var hΔτ Lookup.here
   · have hs : Subst.lift σ j.succ = (σ j).weaken := by simp [Subst.lift]
     rw [hs, Tm.weaken_subst]
     exact WfTm.weaken (hσ hj) hΔτ
@@ -19,68 +19,43 @@ theorem Subst.WellTyped.lift2 {σ : Subst n m} (hσ : Subst.WellTyped σ Γ Δ) 
     Subst.WellTyped (Subst.lift (Subst.lift σ)) (Γ ∷ τ ∷ υ) (Δ ∷ τ.subst σ ∷ υ.subst σ.lift) :=
   Subst.WellTyped.lift (Subst.WellTyped.lift hσ hΔτ) hΔτυ
 
-mutual
-theorem WfTm.subst (ht : Γ ⊢ t ∶ τ) (hΔ : ⊢ Δ) (hσ : Subst.WellTyped σ Γ Δ)
-  : (Δ ⊢ t.subst σ ∶ τ.subst σ) := match ht with
-  | .var hΓ hlook => hσ hlook
-  | .conv ht hσwf hτσ =>
-      .conv (WfTm.subst ht hΔ hσ) (WfTm.subst hσwf hΔ hσ) (DefEq.subst hτσ hΔ hσ)
-  | .pi hτ hυ =>
-      let hτ' := WfTm.subst hτ hΔ hσ
-      .pi hτ' (WfTm.subst hυ (hΔ.cons hτ') (hσ.lift (hΔ.cons hτ')))
-  | .lam hτ hσwf ht =>
-      let hτ' := WfTm.subst hτ hΔ hσ
-      .lam hτ' (WfTm.subst hσwf (hΔ.cons hτ') (hσ.lift (hΔ.cons hτ')))
-        (WfTm.subst ht (hΔ.cons hτ') (hσ.lift (hΔ.cons hτ')))
-  | .app ht hs => by
-      simp
-      exact WfTm.app (WfTm.subst ht hΔ hσ) (WfTm.subst hs hΔ hσ)
-  | .id hτ ha hb =>
-      .id (WfTm.subst hτ hΔ hσ) (WfTm.subst ha hΔ hσ) (WfTm.subst hb hΔ hσ)
-  | .refl ha => .refl (WfTm.subst ha hΔ hσ)
-  | .j hτ hIdT hC hp hd => by
-      have hτ' := WfTm.subst hτ hΔ hσ
-      have hΔτ := hΔ.cons hτ'
-      have hIdT' := WfTm.subst hIdT hΔτ (hσ.lift hΔτ)
-      have hΔτId := hΔτ.cons hIdT'
-      have hC' := WfTm.subst hC hΔτId (hσ.lift2 hΔτ hΔτId)
-      have hd' := WfTm.subst hd hΔ hσ
-      simp only [Tm.subst, Tm.subst1_subst, Tm.weaken_subst, Subst.lift, Fin.cases_zero]
-        at hIdT' hC' hd' ⊢
-      exact WfTm.j hτ' hIdT' hC' (WfTm.subst hp hΔ hσ) hd'
-  | .u hΓ => .u hΔ
-
 theorem DefEq.subst (heq : Γ ⊢ t₁ ≡ t₂ ∶ τ) (hΔ : ⊢ Δ) (hσ : Subst.WellTyped σ Γ Δ)
   : (Δ ⊢ t₁.subst σ ≡ t₂.subst σ ∶ τ.subst σ) := match heq with
-  | .refl ht => .refl (WfTm.subst ht hΔ hσ)
+  | .var _ hlook => hσ hlook
+  | .u _ => .u hΔ
   | .symm h => .symm (DefEq.subst h hΔ hσ)
   | .trans h₁ h₂ => .trans (DefEq.subst h₁ hΔ hσ) (DefEq.subst h₂ hΔ hσ)
-  | .pi hτwf hτ hυ =>
-      let hτ' := WfTm.subst hτwf hΔ hσ
-      .pi hτ' (DefEq.subst hτ hΔ hσ) (DefEq.subst hυ (hΔ.cons hτ') (hσ.lift (hΔ.cons hτ')))
-  | .lam hτ hσwf hτeq ht =>
-      let hτ' := WfTm.subst hτ hΔ hσ
-      .lam hτ' (WfTm.subst hσwf (hΔ.cons hτ') (hσ.lift (hΔ.cons hτ')))
-        (DefEq.subst hτeq hΔ hσ)
-        (DefEq.subst ht (hΔ.cons hτ') (hσ.lift (hΔ.cons hτ')))
+  | .conv h hσwf hτσ =>
+      .conv (DefEq.subst h hΔ hσ) (DefEq.subst hσwf hΔ hσ) (DefEq.subst hτσ hΔ hσ)
+  | .pi hτ hυ =>
+      let hτ' := DefEq.subst hτ hΔ hσ
+      let hΔτ := hΔ.cons hτ'.wf_left
+      .pi hτ' (DefEq.subst hυ hΔτ (hσ.lift hΔτ))
+  | .lam hσwf hτeq ht =>
+      let hτ' := DefEq.subst hτeq hΔ hσ
+      let hΔτ := hΔ.cons hτ'.wf_left
+      .lam (DefEq.subst hσwf hΔτ (hσ.lift hΔτ)) hτ' (DefEq.subst ht hΔτ (hσ.lift hΔτ))
   | .app ht hm => by
       simp
       exact DefEq.app (DefEq.subst ht hΔ hσ) (DefEq.subst hm hΔ hσ)
-  | .lamβ hlam hm => by
+  | .lamβ hτ hσwf ht hm => by
+      have hτ' := DefEq.subst hτ hΔ hσ
+      have hΔτ := hΔ.cons hτ'
       simp
-      exact DefEq.lamβ (WfTm.subst hlam hΔ hσ) (WfTm.subst hm hΔ hσ)
+      exact DefEq.lamβ hτ' (DefEq.subst hσwf hΔτ (hσ.lift hΔτ))
+        (DefEq.subst ht hΔτ (hσ.lift hΔτ)) (DefEq.subst hm hΔ hσ)
   | .lamη ht => by
       have h0 : Subst.lift σ 0 = Tm.var 0 := by simp [Subst.lift]
       simp [Tm.subst]
       rw [Tm.weaken_subst, h0]
-      exact DefEq.lamη (WfTm.subst ht hΔ hσ)
+      exact DefEq.lamη (DefEq.subst ht hΔ hσ)
   | .id hτeq haeq hbeq =>
       .id (DefEq.subst hτeq hΔ hσ) (DefEq.subst haeq hΔ hσ) (DefEq.subst hbeq hΔ hσ)
   | .reflId hτeq haeq => .reflId (DefEq.subst hτeq hΔ hσ) (DefEq.subst haeq hΔ hσ)
   | .j hτ hIdT hCeq hdeq hpeq => by
-      have hτ' := WfTm.subst hτ hΔ hσ
+      have hτ' := DefEq.subst hτ hΔ hσ
       have hΔτ := hΔ.cons hτ'
-      have hIdT' := WfTm.subst hIdT hΔτ (hσ.lift hΔτ)
+      have hIdT' := DefEq.subst hIdT hΔτ (hσ.lift hΔτ)
       have hΔτId := hΔτ.cons hIdT'
       have hCeq' := DefEq.subst hCeq hΔτId (hσ.lift2 hΔτ hΔτId)
       have hdeq' := DefEq.subst hdeq hΔ hσ
@@ -88,16 +63,15 @@ theorem DefEq.subst (heq : Γ ⊢ t₁ ≡ t₂ ∶ τ) (hΔ : ⊢ Δ) (hσ : Su
         at hIdT' hCeq' hdeq' ⊢
       exact DefEq.j hτ' hIdT' hCeq' hdeq' (DefEq.subst hpeq hΔ hσ)
   | .jβ hτ ha hIdT hC hd => by
-      have hτ' := WfTm.subst hτ hΔ hσ
+      have hτ' := DefEq.subst hτ hΔ hσ
       have hΔτ := hΔ.cons hτ'
-      have hIdT' := WfTm.subst hIdT hΔτ (hσ.lift hΔτ)
+      have hIdT' := DefEq.subst hIdT hΔτ (hσ.lift hΔτ)
       have hΔτId := hΔτ.cons hIdT'
-      have hC' := WfTm.subst hC hΔτId (hσ.lift2 hΔτ hΔτId)
-      have hd' := WfTm.subst hd hΔ hσ
+      have hC' := DefEq.subst hC hΔτId (hσ.lift2 hΔτ hΔτId)
+      have hd' := DefEq.subst hd hΔ hσ
       simp only [Tm.subst, Tm.subst1_subst, Tm.weaken_subst, Subst.lift, Fin.cases_zero]
         at hIdT' hC' hd' ⊢
-      exact DefEq.jβ hτ' (WfTm.subst ha hΔ hσ) hIdT' hC' hd'
-end
+      exact DefEq.jβ hτ' (DefEq.subst ha hΔ hσ) hIdT' hC' hd'
 
 theorem Subst.WellTyped.single (hΓ : ⊢ Γ) (hu : Γ ⊢ u ∶ τ) :
     Subst.WellTyped (Subst.single u) (Γ ∷ τ) Γ := by
@@ -108,12 +82,12 @@ theorem Subst.WellTyped.single (hΓ : ⊢ Γ) (hu : Γ ⊢ u ∶ τ) :
     simpa [Subst.single] using hu
   · show Γ ⊢ Subst.single u j.succ ∶ τ'.weaken [/ u ]
     rw [Tm.weaken_subst1]
-    simpa [Subst.single] using WfTm.var hΓ hj
-
-theorem WfTm.subst1 (ht : Γ ∷ τ ⊢ t ∶ σ) (hv : Γ ⊢ v ∶ τ) (hΓ : ⊢ Γ) :
-    Γ ⊢ t [/ v ] ∶ σ [/ v ] :=
-  WfTm.subst ht hΓ (Subst.WellTyped.single hΓ hv)
+    simpa [Subst.single] using DefEq.var hΓ hj
 
 theorem DefEq.subst1 (heq : Γ ∷ τ ⊢ t₁ ≡ t₂ ∶ σ) (hv : Γ ⊢ v ∶ τ) (hΓ : ⊢ Γ) :
     Γ ⊢ t₁ [/ v ] ≡ t₂ [/ v ] ∶ σ [/ v ] :=
   DefEq.subst heq hΓ (Subst.WellTyped.single hΓ hv)
+
+theorem WfTm.subst1 (ht : Γ ∷ τ ⊢ t ∶ σ) (hv : Γ ⊢ v ∶ τ) (hΓ : ⊢ Γ) :
+    Γ ⊢ t [/ v ] ∶ σ [/ v ] :=
+  DefEq.subst1 ht hv hΓ
