SPos/Typing/Weakening.lean
@@ -20,81 +20,62 @@ theorem Ren.WellTyped.lift2 {r : Ren n m} (hr : Ren.WellTyped r Γ Δ) {τ : Tm 
       (Δ ∷ τ.rename r ∷ υ.rename (Ren.lift r)) :=
   Ren.WellTyped.lift (Ren.WellTyped.lift hr)
 
-mutual
-theorem WfTm.rename (ht : Γ ⊢ t ∶ τ) (hΔ : ⊢ Δ) (hr : Ren.WellTyped r Γ Δ)
-  : (Δ ⊢ t.rename r ∶ τ.rename r) := match ht with
-  | .var hΓ hlook => .var hΔ (hr hlook)
-  | .conv ht hσ hτσ => .conv (WfTm.rename ht hΔ hr) (WfTm.rename hσ hΔ hr) (DefEq.rename hτσ hΔ hr)
-  | .pi hτ hυ => .pi (WfTm.rename hτ hΔ hr) (WfTm.rename hυ (hΔ.cons (WfTm.rename hτ hΔ hr)) hr.lift)
-  | .lam hτ hσ ht => .lam (WfTm.rename hτ hΔ hr)
-      (WfTm.rename hσ (hΔ.cons (WfTm.rename hτ hΔ hr)) hr.lift)
-      (WfTm.rename ht (hΔ.cons (WfTm.rename hτ hΔ hr)) hr.lift)
-  | .app ht hs => by
-      simp
-      exact WfTm.app (WfTm.rename ht hΔ hr) (WfTm.rename hs hΔ hr)
-  | .id hτ ha hb =>
-      .id (WfTm.rename hτ hΔ hr) (WfTm.rename ha hΔ hr) (WfTm.rename hb hΔ hr)
-  | .refl ha => .refl (WfTm.rename ha hΔ hr)
-  | .j hτ hIdT hC hp hd => by
-      have hτ' := WfTm.rename hτ hΔ hr
-      have hIdT' := WfTm.rename hIdT (hΔ.cons hτ') hr.lift
-      have hC' := WfTm.rename hC ((hΔ.cons hτ').cons hIdT') hr.lift2
-      have hd' := WfTm.rename hd hΔ hr
-      simp only [Tm.rename, Tm.subst1_rename, Tm.weaken_rename, Ren.lift, Fin.cases_zero]
-        at hIdT' hC' hd' ⊢
-      exact WfTm.j hτ' hIdT' hC' (WfTm.rename hp hΔ hr) hd'
-  | .u hΓ => .u hΔ
-
 theorem DefEq.rename (heq : Γ ⊢ t ≡ t' ∶ τ) (hΔ : ⊢ Δ) (hr : Ren.WellTyped r Γ Δ)
   : (Δ ⊢ t.rename r ≡ t'.rename r ∶ τ.rename r) := match heq with
-  | .refl ht => .refl (WfTm.rename ht hΔ hr)
+  | .var _ hlook => .var hΔ (hr hlook)
+  | .u _ => .u hΔ
   | .symm h => .symm (DefEq.rename h hΔ hr)
   | .trans h₁ h₂ => .trans (DefEq.rename h₁ hΔ hr) (DefEq.rename h₂ hΔ hr)
-  | .pi hτwf hτ hυ => .pi (WfTm.rename hτwf hΔ hr)
-      (DefEq.rename hτ hΔ hr) (DefEq.rename hυ (hΔ.cons (WfTm.rename hτwf hΔ hr)) hr.lift)
-  | .lam hτ hσ hτeq ht => .lam (WfTm.rename hτ hΔ hr)
-      (WfTm.rename hσ (hΔ.cons (WfTm.rename hτ hΔ hr)) hr.lift)
-      (DefEq.rename hτeq hΔ hr)
-      (DefEq.rename ht (hΔ.cons (WfTm.rename hτ hΔ hr)) hr.lift)
+  | .conv h hσ hτσ =>
+      .conv (DefEq.rename h hΔ hr) (DefEq.rename hσ hΔ hr) (DefEq.rename hτσ hΔ hr)
+  | .pi hτ hυ =>
+      have hτ' := DefEq.rename hτ hΔ hr
+      .pi hτ' (DefEq.rename hυ (hΔ.cons hτ'.wf_left) hr.lift)
+  | .lam hσ hτeq ht =>
+      have hτ' := DefEq.rename hτeq hΔ hr
+      have hΔτ := hΔ.cons hτ'.wf_left
+      .lam (DefEq.rename hσ hΔτ hr.lift) hτ' (DefEq.rename ht hΔτ hr.lift)
   | .app ht hm => by
       simp
       exact DefEq.app (DefEq.rename ht hΔ hr) (DefEq.rename hm hΔ hr)
-  | .lamβ hlam hm => by
+  | .lamβ hτ hσ ht hm => by
+      have hτ' := DefEq.rename hτ hΔ hr
+      have hΔτ := hΔ.cons hτ'
       simp
-      exact DefEq.lamβ (WfTm.rename hlam hΔ hr) (WfTm.rename hm hΔ hr)
+      exact DefEq.lamβ hτ' (DefEq.rename hσ hΔτ hr.lift) (DefEq.rename ht hΔτ hr.lift)
+        (DefEq.rename hm hΔ hr)
   | .lamη ht => by
       have h0 : Ren.lift r 0 = 0 := by simp [Ren.lift]
       simp [Tm.rename]
       rw [h0]
-      exact DefEq.lamη (WfTm.rename ht hΔ hr)
+      exact DefEq.lamη (DefEq.rename ht hΔ hr)
   | .id hτeq haeq hbeq =>
       .id (DefEq.rename hτeq hΔ hr) (DefEq.rename haeq hΔ hr) (DefEq.rename hbeq hΔ hr)
   | .reflId hτeq haeq => .reflId (DefEq.rename hτeq hΔ hr) (DefEq.rename haeq hΔ hr)
   | .j hτ hIdT hCeq hdeq hpeq => by
-      have hτ' := WfTm.rename hτ hΔ hr
-      have hIdT' := WfTm.rename hIdT (hΔ.cons hτ') hr.lift
-      have hCeq' := DefEq.rename hCeq ((hΔ.cons hτ').cons hIdT') hr.lift2
+      have hτ' := DefEq.rename hτ hΔ hr
+      have hIdT' := DefEq.rename hIdT (hΔ.cons hτ') hr.lift
+      have hCeq' := DefEq.rename hCeq ((hΔ.cons hτ').cons hIdT'.wf_left) hr.lift2
       have hdeq' := DefEq.rename hdeq hΔ hr
       simp only [Tm.rename, Tm.subst1_rename, Tm.weaken_rename, Ren.lift, Fin.cases_zero]
         at hIdT' hCeq' hdeq' ⊢
       exact DefEq.j hτ' hIdT' hCeq' hdeq' (DefEq.rename hpeq hΔ hr)
   | .jβ hτ ha hIdT hC hd => by
-      have hτ' := WfTm.rename hτ hΔ hr
-      have hIdT' := WfTm.rename hIdT (hΔ.cons hτ') hr.lift
-      have hC' := WfTm.rename hC ((hΔ.cons hτ').cons hIdT') hr.lift2
-      have hd' := WfTm.rename hd hΔ hr
+      have hτ' := DefEq.rename hτ hΔ hr
+      have hIdT' := DefEq.rename hIdT (hΔ.cons hτ') hr.lift
+      have hC' := DefEq.rename hC ((hΔ.cons hτ').cons hIdT'.wf_left) hr.lift2
+      have hd' := DefEq.rename hd hΔ hr
       simp only [Tm.rename, Tm.subst1_rename, Tm.weaken_rename, Ren.lift, Fin.cases_zero]
         at hIdT' hC' hd' ⊢
-      exact DefEq.jβ hτ' (WfTm.rename ha hΔ hr) hIdT' hC' hd'
-end
+      exact DefEq.jβ hτ' (DefEq.rename ha hΔ hr) hIdT' hC' hd'
 
 theorem Ren.succ_wellTyped (Γ : Ctx n) (σ : Tm n) :
     Ren.WellTyped Fin.succ Γ (Γ ∷ σ) :=
   fun hlook => Lookup.there hlook
 
-theorem WfTm.weaken (ht : Γ ⊢ t ∶ τ) (hΓσ : ⊢ Γ ∷ σ) : Γ ∷ σ ⊢ ↑ t ∶ ↑ τ:=
-  WfTm.rename ht hΓσ (Ren.succ_wellTyped Γ σ)
-
 theorem DefEq.weaken (heq : Γ ⊢ t₁ ≡ t₂ ∶ τ) (hΓσ : ⊢ Γ ∷ σ) :
     Γ ∷ σ ⊢ t₁.weaken ≡ t₂.weaken ∶ τ.weaken :=
   DefEq.rename heq hΓσ (Ren.succ_wellTyped Γ σ)
+
+theorem WfTm.weaken (ht : Γ ⊢ t ∶ τ) (hΓσ : ⊢ Γ ∷ σ) : Γ ∷ σ ⊢ ↑ t ∶ ↑ τ :=
+  DefEq.weaken ht hΓσ
